src/Reflection/InlineInterp.v
@@ -27,27 +27,62 @@ Section language.
 
   Local Hint Extern 1 => eapply interpf_SmartVarVarf.
 
-  Local Ltac t_fin :=
-    repeat match goal with
-           | _ => reflexivity
-           | _ => progress simpl in *
-           | _ => progress unfold postprocess_for_const in *
-           | _ => progress intros
-           | _ => progress inversion_sigma
-           | _ => progress inversion_prod
-           | _ => solve [ intuition eauto ]
-           | _ => apply (f_equal (interp_op _ _ _))
-           | _ => apply (f_equal2 (@pair _ _))
-           | _ => progress specialize_by assumption
-           | _ => progress subst
-           | [ H : context[List.In _ (_ ++ _)] |- _ ] => setoid_rewrite List.in_app_iff in H
-           | [ H : or _ _ |- _ ] => destruct H
-           | _ => progress break_match
-           | _ => rewrite <- !surjective_pairing
-           | [ H : ?x = _, H' : context[?x] |- _ ] => rewrite H in H'
-           | [ H : _ |- _ ] => apply H
-           | [ H : _ |- _ ] => rewrite H
-           end.
+  Local Ltac t_fin_step :=
+    match goal with
+    | _ => reflexivity
+    | _ => progress simpl in *
+    | _ => progress unfold postprocess_for_const in *
+    | _ => progress intros
+    | _ => progress inversion_sigma
+    | _ => progress inversion_prod
+    | _ => solve [ intuition eauto ]
+    | _ => apply (f_equal (interp_op _ _ _))
+    | _ => apply (f_equal2 (@pair _ _))
+    | _ => progress specialize_by assumption
+    | _ => progress subst
+    | [ H : context[List.In _ (_ ++ _)] |- _ ] => setoid_rewrite List.in_app_iff in H
+    | [ H : _ = _ :> inline_directive _ |- _ ]
+      => apply (f_equal exprf_of_inline_directive) in H
+    | [ H : exprf_of_inline_directive _ = _ |- _ ]
+      => apply (f_equal (interpf interp_op)) in H
+    | [ H : @fst ?A ?B ?x = _, H' : context H'T[@fst ?A' ?B' ?x] |- _ ]
+      => let H'T' := context H'T[@fst A B x] in
+         progress change H'T' in H'
+    | [ H : @snd ?A ?B ?x = _, H' : context H'T[@snd ?A' ?B' ?x] |- _ ]
+      => let H'T' := context H'T[@snd A B x] in
+         progress change H'T' in H'
+    | [ H : or _ _ |- _ ] => destruct H
+    | _ => progress break_match
+    | _ => rewrite <- !surjective_pairing
+    | [ H : ?x = _, H' : context[?x] |- _ ] => rewrite H in H'
+    | [ H : _ |- _ ] => rewrite H; []
+    | [ H : _, H' : _ |- _ ] => rewrite H in H' by fail
+    | [ H : _ |- _ ] => apply H; solve [ repeat t_fin_step ]
+    | [ H : _ |- _ ] => rewrite H; solve [ repeat t_fin_step ]
+    end.
+  Local Ltac t_fin := repeat t_fin_step.
+
+  Lemma interpf_inline_const_genf postprocess G {t} e1 e2
+        (wf : @wff _ _ G t e1 e2)
+        (Hpostprocess : forall t e, interpf interp_op (exprf_of_inline_directive (postprocess t e)) = interpf interp_op e)
+        (H : forall t x x',
+            List.In
+              (existT (fun t : base_type_code => (exprf (Tbase t) * interp_base_type t)%type) t
+                      (x, x')) G
+            -> interpf interp_op x = x')
+    : interpf interp_op (inline_const_genf postprocess e1) = interpf interp_op e2.
+  Proof.
+    clear -wf H Hpostprocess.
+    induction wf; t_fin.
+  Qed.
+
+  Lemma interpf_postprocess_for_const is_const t e
+    : interpf interp_op (exprf_of_inline_directive (postprocess_for_const is_const t e)) = interpf interp_op e.
+  Proof.
+    unfold postprocess_for_const; t_fin.
+  Qed.
+
+  Local Hint Resolve interpf_postprocess_for_const.
 
   Lemma interpf_inline_constf is_const G {t} e1 e2
         (wf : @wff _ _ G t e1 e2)
@@ -57,12 +92,32 @@ Section language.
                       (x, x')) G
             -> interpf interp_op x = x')
     : interpf interp_op (inline_constf is_const e1) = interpf interp_op e2.
-  Proof.
-    clear -wf H.
-    induction wf; t_fin.
-  Qed.
+  Proof. eapply interpf_inline_const_genf; eauto. Qed.
 
   Local Hint Resolve interpf_inline_constf.
+
+  Lemma interp_inline_const_gen postprocess G {t} e1 e2
+        (wf : @wf _ _ G t e1 e2)
+        (H : forall t x x',
+            List.In
+              (existT (fun t : base_type_code => (exprf (Tbase t) * interp_base_type t)%type) t
+                      (x, x')) G
+            -> interpf interp_op x = x')
+        (Hpostprocess : forall t e, interpf interp_op (exprf_of_inline_directive (postprocess t e)) = interpf interp_op e)
+    : interp_type_gen_rel_pointwise (fun _ => @eq _)
+                                    (interp interp_op (inline_const_gen postprocess e1))
+                                    (interp interp_op e2).
+  Proof.
+    induction wf.
+    { eapply (interpf_inline_const_genf postprocess); eauto. }
+    { simpl in *; intro.
+      match goal with
+      | [ H : _ |- _ ]
+        => apply H; intuition (inversion_sigma; inversion_prod; subst; eauto)
+      end. }
+  Qed.
+
+  Local Hint Resolve interp_inline_const_gen.
 
   Lemma interp_inline_const is_const G {t} e1 e2
         (wf : @wf _ _ G t e1 e2)
@@ -75,13 +130,18 @@ Section language.
                                     (interp interp_op (inline_const is_const e1))
                                     (interp interp_op e2).
   Proof.
-    induction wf.
-    { eapply (interpf_inline_constf is_const); eauto. }
-    { simpl in *; intro.
-      match goal with
-      | [ H : _ |- _ ]
-        => apply H; intuition (inversion_sigma; inversion_prod; subst; eauto)
-      end. }
+    eapply interp_inline_const_gen; eauto.
+  Qed.
+
+  Lemma Interp_InlineConstGen postprocess {t} (e : Expr t)
+        (wf : Wf e)
+        (Hpostprocess : forall t e, interpf interp_op (exprf_of_inline_directive (postprocess _ t e)) = interpf interp_op e)
+    : interp_type_gen_rel_pointwise (fun _ => @eq _)
+                                    (Interp interp_op (InlineConstGen postprocess e))
+                                    (Interp interp_op e).
+  Proof.
+    unfold Interp, InlineConst.
+    eapply (interp_inline_const_gen (postprocess _)); simpl in *; intuition (simpl in *; intuition eauto).
   Qed.
 
   Lemma Interp_InlineConst is_const {t} (e : Expr t)
@@ -90,7 +150,6 @@ Section language.
                                     (Interp interp_op (InlineConst is_const e))
                                     (Interp interp_op e).
   Proof.
-    unfold Interp, InlineConst.
-    eapply (interp_inline_const is_const) with (G := nil); simpl; intuition.
+    eapply Interp_InlineConstGen; eauto.
   Qed.
 End language.
